###### tags: `IM2009 Algorithms` `Homework`
# Algorithms Homework Assignment #3
B08705034 資管二 施芊羽
## Problem 1
Substitute $f(n) = \log_2  {n}$, $c = a$, $a = 2^b$ in the  given theorem, then we can have $$(\log_2 n)^a = o((2^b)^{\log_2{n}}) = o(n^b)$$. 
Hence, we can prove that $(\log_2{n})^a = o(n^b)$ for any constant $a, b \gt 0$. 


## Problem 2
### ( a )
$f(n) = (\log{n})^{\log{n}}$ and $g(n) = \frac{n}{\log{n}}$
1. $f(n) = O(g(n))$
If $f(n) = O(g(n))$, then $f(n) = \omega(g(n))$ will not be satisfied. However:
$\lim_{n \rightarrow \infty}{\frac{\frac{n}{\log{n}}}{(\log{n})^{\log{n}}}} \\= \lim_{n \rightarrow \infty} \frac{n}{\log{n} \space {(\log{n})^{\log{n}}}}\\= \lim_{n \rightarrow \infty} {\frac{n}{\log{n}^{\log{n} + 1}}} \\= \lim_{n \rightarrow \infty} {\frac{1}{\log{n} \space \frac{1}{n}\log{e}}} \quad\text{Use L^Hopital's Rule} \\= 0$
Then $\lim_{n \rightarrow \infty} {\frac{g(n)}{f(n)}} = 0$, so $f(n) = \omega(g(n))$, hence, $f(n) \ne O(g(n))$
2. $f(n) = \Omega(g(n))$
Claim $f(n) = \Omega(g(n))$, then there exist $c, N$ such that $\forall n \ge N, c \in N$: let $c = 1$, then $(\log{n})^{\log{n}} \ge c \dot (\frac{n}{\log{n}}) \\ \Rightarrow x^x \ge c (\frac{2^x}{x}) \quad(\text{let }x = \log{n} )\\ \Rightarrow x \log{x} \ge x + \log{c} - \log{x} \quad (\text{take }\log_2\text{ at each side})$ 
(when $x \gt 1$, it satisfies $\Rightarrow n \gt 2$)
Hence, when $n \gt 2, c = 1$, then $f(n) = \Omega(\log{n})$

### ( b )
$f(n) = n^3 2^n$ and $g(n) = 3^n$
1. $f(n) = O(g(n))$
If $f(n) = O(g(n))$, then there exist $c$ and $N$, such that $\forall n \ge N, f(n) \le cg(n)$. 
Let $c = 1$:
$n^2 2^n \le c3^n \\ \leftarrow n^2 \le c(\frac{3}{2})^n \\ \leftarrow 2 \log{n} \le n(\log{3} - \log{2}) + \log{c} \quad \text{take } \log_2 \text{ from each side}\\ \leftarrow 2 \log{n} \le 0.585 n$
When $n = 13$, $2 \log 3 \sim 7.4 \le 0.585 \times {13} \sim 7.6$. Hence, we can find that when $c = 1$, $n \ge 13$, $n^2 2^n \le c 3^n$, therefore, $f(n) = O(g(n))$.
2. $f(n) = \Omega(g(n))$
If $f(n) = \Omega(g(n))$, then $f(n) = o(g(n))$ will not be satisfied. However:
$\lim_{n \rightarrow \infty}{\frac{n^2 2^n}{3^n}} \\ = \lim_{n \rightarrow \infty}{\frac{n^2}{(\frac{3}{2})^n}} \\ = \lim_{n \rightarrow \infty}{\frac{2n}{\ln(\frac{3}{2})(\frac{3}{2})^n}} \quad \text{By L'Hopital's Rule}\\ = \lim_{n \rightarrow \infty}{\frac{2}{(\ln{\frac{3}{2}})^2 (\frac{3}{2})^n}} \quad \text{By L'Hopital's Rule}\\ = 0$
Then we can know that $\lim_{n \rightarrow \infty}{\frac{n^2 2^n}{3^n}} = \lim_{n \rightarrow \infty}{\frac{f(n)}{g(n)}} = 0$, therefore, $f(n) = o(g(n))$. Hence, we can know that $f(n) \ne \Omega(g(n))$


## Problem 3
If we know that $f(n) = O(g(n))$, which means for a constant $c$ and $N$, when $n \ge N$, then $f(n) \le c \times g(n)$. :
$f(n) \le c \times g(n) \quad \text{for } n \gt N \\ \rightarrow \log{f(n)} \le \log{(c \times g(n))} \\
\rightarrow \log{f(n)} \le \log{c} + \log{g(n)}$
Hence, we need to find $c' \ge c$ such that $\log{f(n)} \le \log{c} + \log{g(n)} \le c' \times \log{g(n)}$ for $n \gt N$. 
Since $\log{c}$ is a constant under the suppose, we are able to find the $c'$ which makes the statement holds then we can have $c'$ and $N$ to prove $\log{f(n)} \le c' \times \log{g(n)}$ for $n \gt N$, hence, we can said that $\log{f(n)} = O(\log{g(n)}).$ 
It'll also be true for $2^{f(n)} = O(2^{g(n)})$, as we've done above we know that $f(n) \le c \times g(n)$ then $2^{f(n)} \le 2^{c \times g(n)} = 2^c \times 2^{g(n)}$ for all $n \gt N$. In this case, we can have $c'' = 2^c$ and $N = N$, which will make $2^{f(n)} \le c'' \times 2^{g(n)}$ for all $n \gt N$. Therefore, $2^{f(n)} = O(2^{g(n)})$ is true. 
If $f(n)$ is a constant the suppose $f(n)$ is a strictly increasing function will not be justified, however if we can find $g(n)$ that makes $f(n) = O(g(n))$ the statement above can still be held. 


## Problem 4
We know that:
$T(n) = n + \sum_{i = 1}^{n - 1} {T(i)} = n + T(n - 1) + \sum_{i = 1}^{n - 2} {T(i)}$
$T(n - 1) = n - 1 + \sum_{i = 1}^{n - 2} {T(i)}$
Then we can get:
$T(n) - T(n - 1) = (n + T(n - 1) + \sum_{i = 1}^{n - 2} {T(i)}) - (n - 1 + \sum_{i = 1}^{n - 2} {T(i)}) = T(n - 1) + 1 \\ \Rightarrow T(n) = 2T(n - 1) + 1 \\ = 2^1(2T(n - 2) + 1) + 1 \\= 2^2(2T(n - 3) + 1) + 2 + 1 \\ = 2^3 T(n - 3) + 2^2 + 2^1 + 2^0 \\= 2^x T(n - x) + \sum_{i = 0}^{x - 1}2^i \\ = \space ...... \\= 2^{(n - 1)} T(n - (n - 1)) + \sum_{i = 0}^{n - 2} 2^i = 2^{(n-1)}T(1) + \sum_{i = 0}^{n - 2} 2^i \\= 2^{(n - 1)} + \frac{1 \times (2^{(n-1)} - 1)}{2 - 1} \quad\text{(Sum of Geometric Sequence)} \\ = 2^{(n - 1)} + 2^{(n - 1)} - 1 = 2^n - 1$
Hence, we can solve the recurrence relation that $T(n) = 2^n - 1$.


## Problem 5
Assume that $n$ is a power of $2$, which means $n = 2^k, k\in N$, then we can solve:
$T(n) = T(2^k) = 2T(\frac{n}{2}) + 1 \\= 2\times T(2^{k - 1}) + 1 \\=2 \times (2 \times T(2^{k - 2}) + 1) + 1 \\= 2^2 \times T(2^{k - 2}) + 2 + 1 \\= 2^i \times T(2^{k - i}) + \sum_{j = 0}^{i - 1} 2^j \\ = 2^{k - 1} \times T(2^{k - (k - 1)}) + \sum_{j = 0}^{k - 2} 2^j \\= 2^{k - 1} \times T(2^1) + \frac{1 \times (2^{k - 1} - 1)}{2 - 1} = 2^{k - 1} \times {1} + 2^{k - 1} - 1= 2^{k} - 1= n - 1$

Since we know that $T(n) = n - 1$ for $n$ is a power of $2$, we can still suppose that $T(n) = O(n)$, thus, there exists $c$ and $N$ such that $T(n) = n - 1 \le cn$ for $n \gt N$. However, we have no way to eliminate the positive constant in the case since we need to accumlate it in the recursion. Hence, we take a guess $T(n) \le cn - 1$, then $T(\frac{n}{2}) \le c(\frac{n}{2}) - 1$. Therefore, we can prove that:
$T(n) = 2 T(\frac{n}{2}) + 1 \le 2 (c(\frac{n}{2}) - 1) + 1 = cn - 1 \le cn$. 
To sum up, we can prove that $T(n) = O(n)$ because $T(n) \le cn$. 